Loom/Triple/Gadget.lean
@@ -13,7 +13,7 @@ set_option linter.unusedVariables false in
 def assertGadget (name : Name) (as : l) : m PUnit := pure ⟨⟩
 
 theorem Spec.assertGadget (name : Name) (as : l) [Frame l] :
-  Triple (m := m) (as ⊓ ((name : as) ⇨ post ⟨⟩)) (Loom.assertGadget name as) post epost := by
+  Triple (m := m) (as ⊓ (as ⇨ post ⟨⟩)) (Loom.assertGadget name as) post epost := by
   simpa [Loom.assertGadget] using
     (Triple.pure (m := m) (pre := as ⊓ himp as (post ⟨⟩)) (post := post) (epost := epost)
       (a := ⟨⟩) (h := himp_sound (a := as) (b := post ⟨⟩)))
